examples/case_studies/proc.bpl
@@ -1,8 +1,10 @@
-procedure max(x: int, y: int) returns (z: int) {
+procedure test(x: int, y: int) returns (z: int) {
     assume x > y;
     z := x;
     assert z > y;
+}
 
+procedure loop1() {
     var a: int, b: int;
 
     var a0: int, b0: int := a, b;
@@ -18,4 +20,23 @@ procedure max(x: int, y: int) returns (z: int) {
 
     assert b == a0 + b0;
 }
+
+procedure summary1() {
+    var a: int, b: int;
+
+    var a0: int, b0: int := a, b;
+    assume a >= 0;
+
+    while(a > 0)
+        decreases a;
+        invariant a >= 0;
+        summary   b == old(a + b);
+    {
+        a := a - 1;
+        b := b + 1;
+    }
+
+    assert b == a0 + b0;
+}
+
 
